adding a preorder to the ghost state

src/dice/HWState.fst
@@ -1,3 +1,15 @@
 module HWState
 
+module G = FStar.Ghost
+
 let t = bool & bool
+
+let t_rel = fun s1 s2 ->
+  Seq.length s1 == Seq.length s2 /\
+  (Seq.length s1 > 0 ==>
+    (let t1 = G.reveal (Seq.index s1 0) in
+     let t2 = G.reveal (Seq.index s2 0) in
+     match t1, t2 with
+     | (true, _), (false, _)
+     | (false, _), (false, true) -> True
+     | _ -> if t1 = t2 then True else False))
